Weidenbach_Book/CDCL_Extensions/DPLL_W_Partial_Encoding.thy
@@ -45,6 +45,194 @@ locale dpll_optimal_encoding =
 begin
 
 
+inductive odecide :: \<open>'st \<Rightarrow> 'st \<Rightarrow> bool\<close> where
+  odecide_noweight: \<open>odecide S T\<close>
+if
+  \<open>undefined_lit (trail S) L\<close> and
+  \<open>atm_of L \<in> atms_of_mm (clauses S)\<close> and
+  \<open>T \<sim> cons_trail (Decided L) S\<close> and
+  \<open>atm_of L \<in> \<Sigma> - \<Delta>\<Sigma>\<close> |
+  odecide_replacement_pos: \<open>odecide S T\<close>
+if
+  \<open>undefined_lit (trail S) (Pos (replacement_pos L))\<close> and
+  \<open>T \<sim> cons_trail (Decided (Pos (replacement_pos L))) S\<close> and
+  \<open>L \<in> \<Delta>\<Sigma>\<close> |
+  odecide_replacement_neg: \<open>odecide S T\<close>
+if
+  \<open>undefined_lit (trail S) (Pos (replacement_neg L))\<close> and
+  \<open>T \<sim> cons_trail (Decided (Pos (replacement_neg L))) S\<close> and
+  \<open>L \<in> \<Delta>\<Sigma>\<close>
+
+inductive_cases odecideE: \<open>odecide S T\<close>
+
+inductive dpll_conflict :: \<open>'st \<Rightarrow> 'st \<Rightarrow> bool\<close> where
+\<open>dpll_conflict S S\<close>
+if \<open>C \<in># clauses S\<close> and
+  \<open>trail S \<Turnstile>as CNot C\<close>
+
+inductive odpll\<^sub>W_core_stgy :: "'st \<Rightarrow> 'st \<Rightarrow> bool" for S T where
+propagate: "dpll_propagate S T \<Longrightarrow> odpll\<^sub>W_core_stgy S T" |
+decided: "odecide S T \<Longrightarrow> no_step dpll_propagate S  \<Longrightarrow> no_step dpll_backtrack S \<Longrightarrow>
+  no_step dpll_conflict S \<Longrightarrow> odpll\<^sub>W_core_stgy S T " |
+backtrack: "dpll_backtrack S T \<Longrightarrow> odpll\<^sub>W_core_stgy S T" |
+backtrack_opt: \<open>bnb.backtrack_opt S T \<Longrightarrow> odpll\<^sub>W_core_stgy S T\<close>
+
+lemma odpll\<^sub>W_core_stgy_clauses:
+  \<open>odpll\<^sub>W_core_stgy S T \<Longrightarrow> clauses T = clauses S\<close>
+  by (induction rule: odpll\<^sub>W_core_stgy.induct)
+   (auto simp: dpll_propagate.simps odecide.simps dpll_backtrack.simps
+      bnb.backtrack_opt.simps)
+
+lemma rtranclp_odpll\<^sub>W_core_stgy_clauses:
+  \<open>odpll\<^sub>W_core_stgy\<^sup>*\<^sup>* S T \<Longrightarrow> clauses T = clauses S\<close>
+  by (induction rule: rtranclp_induct)
+    (auto dest: odpll\<^sub>W_core_stgy_clauses)
+
+
+inductive odpll\<^sub>W_bnb_stgy :: \<open>'st \<Rightarrow> 'st \<Rightarrow> bool\<close> for S T :: 'st where
+dpll:
+  \<open>odpll\<^sub>W_bnb_stgy S T\<close>
+  if \<open>odpll\<^sub>W_core_stgy S T\<close> |
+bnb:
+  \<open>odpll\<^sub>W_bnb_stgy S T\<close>
+  if \<open>bnb.dpll\<^sub>W_bound S T\<close>
+
+lemma odpll\<^sub>W_bnb_stgy_clauses:
+  \<open>odpll\<^sub>W_bnb_stgy S T \<Longrightarrow> clauses T = clauses S\<close>
+  by (induction rule: odpll\<^sub>W_bnb_stgy.induct)
+   (auto simp: bnb.dpll\<^sub>W_bound.simps dest: odpll\<^sub>W_core_stgy_clauses)
+
+lemma rtranclp_odpll\<^sub>W_bnb_stgy_clauses:
+  \<open>odpll\<^sub>W_bnb_stgy\<^sup>*\<^sup>* S T \<Longrightarrow> clauses T = clauses S\<close>
+  by (induction rule: rtranclp_induct)
+    (auto dest: odpll\<^sub>W_bnb_stgy_clauses)
+
+lemma odecide_dpll_decide_iff:
+  assumes \<open>clauses S = penc N\<close> \<open>atms_of_mm N = \<Sigma>\<close>
+  shows \<open>odecide S T \<Longrightarrow> dpll_decide S T\<close>
+    \<open>dpll_decide S T \<Longrightarrow> Ex(odecide S)\<close>
+  using assms atms_of_mm_penc_subset2[of N] \<Delta>\<Sigma>_\<Sigma>
+  unfolding odecide.simps dpll_decide.simps
+  apply (auto simp: odecide.simps dpll_decide.simps)
+  apply (metis defined_lit_Pos_atm_iff state_eq_ref)+
+  done
+
+lemma
+  assumes \<open>clauses S = penc N\<close> \<open>atms_of_mm N = \<Sigma>\<close>
+  shows
+    odpll\<^sub>W_core_stgy_dpll\<^sub>W_core_stgy: \<open>odpll\<^sub>W_core_stgy S T \<Longrightarrow> bnb.dpll\<^sub>W_core_stgy S T\<close>
+  using odecide_dpll_decide_iff[OF assms]
+  by (auto simp: odpll\<^sub>W_core_stgy.simps bnb.dpll\<^sub>W_core_stgy.simps)
+
+lemma
+  assumes \<open>clauses S = penc N\<close> \<open>atms_of_mm N = \<Sigma>\<close>
+  shows
+    odpll\<^sub>W_bnb_stgy_dpll\<^sub>W_bnb_stgy: \<open>odpll\<^sub>W_bnb_stgy S T \<Longrightarrow> bnb.dpll\<^sub>W_bnb S T\<close>
+  using odecide_dpll_decide_iff[OF assms]
+  by (auto simp: odpll\<^sub>W_bnb_stgy.simps bnb.dpll\<^sub>W_bnb.simps dest: odpll\<^sub>W_core_stgy_dpll\<^sub>W_core_stgy[OF assms]
+    bnb.dpll\<^sub>W_core_stgy_dpll\<^sub>W_core)
+
+lemma
+  assumes \<open>clauses S = penc N\<close> and [simp]: \<open>atms_of_mm N = \<Sigma>\<close>
+  shows
+    rtranclp_odpll\<^sub>W_bnb_stgy_dpll\<^sub>W_bnb_stgy: \<open>odpll\<^sub>W_bnb_stgy\<^sup>*\<^sup>* S T \<Longrightarrow> bnb.dpll\<^sub>W_bnb\<^sup>*\<^sup>* S T\<close>
+  using assms(1) apply -
+  apply (induction rule: rtranclp_induct)
+  subgoal by auto
+  subgoal for T U
+    using odpll\<^sub>W_bnb_stgy_dpll\<^sub>W_bnb_stgy[of T N U] rtranclp_odpll\<^sub>W_bnb_stgy_clauses[of S T]
+    by auto
+  done
+
+(*
+lemma no_step_odpll\<^sub>W_core_stgy_no_step_dpll\<^sub>W_core_stgy:
+  assumes \<open>clauses S = penc N\<close> and [simp]:\<open>atms_of_mm N = \<Sigma>\<close>
+  shows
+    \<open>no_step odpll\<^sub>W_core_stgy S \<longleftrightarrow> no_step bnb.dpll\<^sub>W_core_stgy S\<close>
+  using odecide_dpll_decide_iff[of S, OF assms]
+  by (auto simp: odpll\<^sub>W_core_stgy.simps bnb.dpll\<^sub>W_core_stgy.simps)
+
+lemma no_step_odpll\<^sub>W_bnb_stgy_no_step_dpll\<^sub>W_bnb:
+  assumes \<open>clauses S = penc N\<close> and [simp]:\<open>atms_of_mm N = \<Sigma>\<close>
+  shows
+    \<open>no_step odpll\<^sub>W_bnb_stgy S \<longleftrightarrow> no_step bnb.dpll\<^sub>W_bnb S\<close>
+  using no_step_odpll\<^sub>W_core_stgy_no_step_dpll\<^sub>W_core_stgy[of S, OF assms] bnb.no_step_stgy_iff
+  by (auto simp: odpll\<^sub>W_bnb_stgy.simps bnb.dpll\<^sub>W_bnb.simps dest: odpll\<^sub>W_core_stgy_dpll\<^sub>W_core_stgy[OF assms]
+    bnb.dpll\<^sub>W_core_stgy_dpll\<^sub>W_core)
+
+lemma full_odpll\<^sub>W_core_stgy_full_dpll\<^sub>W_core_stgy:
+  assumes \<open>clauses S = penc N\<close> and [simp]:\<open>atms_of_mm N = \<Sigma>\<close>
+  shows
+    \<open>full odpll\<^sub>W_bnb_stgy S T \<Longrightarrow> full bnb.dpll\<^sub>W_bnb S T\<close>
+  using no_step_odpll\<^sub>W_bnb_stgy_no_step_dpll\<^sub>W_bnb[of T, OF _ assms(2)]
+    rtranclp_odpll\<^sub>W_bnb_stgy_clauses[of S T, symmetric, unfolded assms]
+    rtranclp_odpll\<^sub>W_bnb_stgy_dpll\<^sub>W_bnb_stgy[of S N T, OF assms]
+   by (auto simp: full_def)
+*)
+
+definition "no_smaller_confl (S ::'st) \<equiv>
+  (\<forall>M K M' D. trail S = M' @ Decided K # M \<longrightarrow> D \<in># clauses S \<longrightarrow> \<not>M \<Turnstile>as CNot D)"
+
+lemma decided_cons_eq_append_decide_cons:
+  "Decided L # Ms = M' @ Decided K # M \<longleftrightarrow>
+    (L = K \<and> Ms = M \<and> M' = []) \<or>
+    (hd M' = Decided L \<and> Ms = tl M' @ Decided K # M \<and> M' \<noteq> [])"
+  by (cases M')
+   auto
+
+lemma [simp]: \<open>T \<sim> S \<Longrightarrow> no_smaller_confl T = no_smaller_confl S\<close>
+  by (auto simp: no_smaller_confl_def)
+
+lemma no_smaller_confl_cons_trail[simp]:
+  \<open>no_smaller_confl (cons_trail (Propagated L C) S) \<longleftrightarrow> no_smaller_confl S\<close>
+  \<open>no_smaller_confl (update_weight_information M' S) \<longleftrightarrow> no_smaller_confl S\<close>
+  by (force simp: no_smaller_confl_def cdcl\<^sub>W_restart_mset.propagated_cons_eq_append_decide_cons)+
+
+lemma no_smaller_confl_cons_trail_decided[simp]:
+  \<open>no_smaller_confl S \<Longrightarrow> no_smaller_confl (cons_trail (Decided L) S) \<longleftrightarrow> (\<forall>C \<in># clauses S. \<not>trail S \<Turnstile>as CNot C)\<close>
+  by (auto simp: no_smaller_confl_def cdcl\<^sub>W_restart_mset.propagated_cons_eq_append_decide_cons
+    decided_cons_eq_append_decide_cons)
+
+
+
+lemma no_step_dpll_backtrack_iff:
+  \<open>no_step dpll_backtrack S \<longleftrightarrow> (count_decided (trail S) = 0 \<or> (\<forall>C \<in># clauses S. \<not>trail S \<Turnstile>as CNot C))\<close>
+  using backtrack_snd_empty_not_decided[of \<open>trail S\<close>] backtrack_split_list_eq[of \<open>trail S\<close>, symmetric]
+  apply (cases \<open>backtrack_split (trail S)\<close>; cases \<open>snd(backtrack_split (trail S))\<close>)
+  by (auto simp: dpll_backtrack.simps count_decided_0_iff)
+
+lemma no_step_dpll_conflict:
+  \<open>(\<forall>S'. \<not> dpll_conflict S S') \<longleftrightarrow> (\<forall>C \<in># clauses S. \<not>trail S \<Turnstile>as CNot C)\<close>
+  by (auto simp: dpll_conflict.simps)
+
+lemma count_decided_0_no_smaller_confl: \<open>count_decided (trail S) = 0 \<Longrightarrow> no_smaller_confl S\<close>
+  by (auto simp: no_smaller_confl_def)
+
+lemma no_smaller_confl_backtrack_split:
+  \<open>no_smaller_confl S \<Longrightarrow>
+       backtrack_split (trail S) = (M', L # M) \<Longrightarrow>
+       no_smaller_confl (reduce_trail_to M S)\<close>
+  using backtrack_split_list_eq[of \<open>trail S\<close>, symmetric]
+  by (auto simp: no_smaller_confl_def)
+  
+lemma odpll\<^sub>W_core_stgy_no_smaller_conflict:
+  \<open>odpll\<^sub>W_core_stgy S T \<Longrightarrow> no_smaller_confl S \<Longrightarrow> no_smaller_confl T\<close>
+  using no_step_dpll_backtrack_iff[of S] apply -
+  by (induction rule: odpll\<^sub>W_core_stgy.induct)
+   (auto simp: cdcl\<^sub>W_restart_mset.propagated_cons_eq_append_decide_cons count_decided_0_no_smaller_confl
+      dpll_propagate.simps dpll_decide.simps odecide.simps decided_cons_eq_append_decide_cons
+      bnb.backtrack_opt.simps dpll_backtrack.simps no_step_dpll_conflict no_smaller_confl_backtrack_split)
+
+lemma odpll\<^sub>W_bound_stgy_no_smaller_conflict: \<open>bnb.dpll\<^sub>W_bound S T \<Longrightarrow> no_smaller_confl S \<Longrightarrow> no_smaller_confl T\<close>
+  by (auto simp: cdcl\<^sub>W_restart_mset.propagated_cons_eq_append_decide_cons count_decided_0_no_smaller_confl
+      dpll_propagate.simps dpll_decide.simps odecide.simps decided_cons_eq_append_decide_cons bnb.dpll\<^sub>W_bound.simps
+      bnb.backtrack_opt.simps dpll_backtrack.simps no_step_dpll_conflict no_smaller_confl_backtrack_split)
+
+lemma odpll\<^sub>W_bnb_stgy_no_smaller_conflict:
+  \<open>odpll\<^sub>W_bnb_stgy S T \<Longrightarrow> no_smaller_confl S \<Longrightarrow> no_smaller_confl T\<close>
+  by (induction rule: odpll\<^sub>W_bnb_stgy.induct)
+    (auto simp: odpll\<^sub>W_core_stgy_no_smaller_conflict odpll\<^sub>W_bound_stgy_no_smaller_conflict)
+
 end
 
 end
